---
title: Third Isomorphism Theorem for Groups
mathjax: true
tags: group-theory
excerpt:
---
\documentclass{article}
%preamble
\usepackage{parskip}
\usepackage{amsmath,amsthm,amssymb}
\usepackage[colorlinks=true]{hyperref}
\newtheorem*{thm}{Third Isomorphism Theorem for Groups}
%\newtheorem{lem}{Lemma}
%\newtheorem{claim}[lem]{Claim}
\theoremstyle{definition}\newtheorem{definition}{Definition}

\begin{document}
	\begin{thm}
		Let $G$ be a group and let $H$ and $K$ be normal subgroups of $G$, with $H \leq K$. Then 
		\begin{enumerate}
			\item $K / H \unlhd G / H$
			\item $( G / H ) / ( K / H ) \cong G / K$
		\end{enumerate}
	\end{thm}
	\begin{proof}
		\
		\begin{enumerate}
			\item $\forall x \in K/H; y \in G/H, \exists k \in K; g \in G : x=kH; y=gH $ and $yxy^{-1}=(gkg^{-1})H$. Since $K$ is a normal subgroup of $G$, $gkg^{-1} \in K$. Thus, $yxy^{-1} \in K/H$ and $K / H \unlhd G / H$
			\item Consider a mapping $\phi : G/H \rightarrow G/K$ by $\phi(gH)=gK$
			
			The map is well-defined since if $aH=bH$, then $a^{-1}b\in H \subseteq K $ and
			$$\phi(aH)=aK \circ (a^{-1}b) K = bK=\phi(bH)$$
			
			The map is homomorphic since $\forall aH, bH \in G/H$, $$\phi(aH)\phi(bH)=(aK)(bK)=(ab)K=\phi((ab)H)$$
			
			It is easy to tell $\phi$ is surjective, so $\operatorname { im } ( \phi )=G/K$. 
			$$\phi(gH)=gK=K \iff g\in K \iff gH \in K/H \implies \operatorname { ker } ( \phi )=K/H $$
			
			Based on First Isomorphism Theorem, $( G / H ) / ( K / H ) \cong G / K$
		\end{enumerate}
	\end{proof}		
\end{document}